src/riscv/Examples/smt/list.smt
@@ -1,0 +1,9 @@
+(declare-datatypes (T) ((Lst nil (cons (hd T) (tl Lst) (foo Int)))))
+
+(define-fun test ((l1 (Lst Int)) (l2 (Lst Int))) (Lst Int)
+  (match l1 (
+    (nil l2)
+    ((cons _ t _) (cons 1 t 2)))))
+
+(check-sat)
+(get-model)
